Progress in splay_proof.v.

test/coq/splay_proof.v
@@ -1,8 +1,79 @@
+Require Import Coq.Wellfounded.Inverse_Image.
 From osiris Require Import osiris.
 From osiris.semantics Require Export evalprime.
 From osiris.proofmode Require Export proofmode. (* TODO *)
 From osiris.libs Require Import Stdlib.
 From test Require Import splay.
+
+(* -------------------------------------------------------------------------- *)
+
+(* WIP *)
+
+Ltac SIMP_specify x φ :=
+  lazymatch goal with
+  | |- SIMP (bind (dconcatenating ?δ _) _) _ =>
+      let o := eval cbn in (lookup_name δ x) in
+      lazymatch o with ret ?v =>
+        let h := fresh in
+        assert (φ v) as h; [| revert h; generalize v ]
+      end
+  end.
+
+Lemma SIMP_simp_bind X Y (_ : Encode Y)
+   m f (x : X) (ψ : Y → Prop) :
+  simp m (ret x) →
+  SIMP (f x) ψ →
+  SIMP (bind m f) ψ.
+  (* This is [@bind X val]. *)
+Proof.
+  intros Hm Hf.
+  destruct Hf as (y & ? & ?).
+  eexists; split; eauto using prove_simp_bind.
+Qed.
+
+Lemma SIMP_covariant `{Encode X} m (φ ψ : X → Prop) :
+  SIMP m φ →
+  (∀ x, φ x → ψ x) →
+  SIMP m ψ.
+Proof.
+  intros (x & Hm & Hx) ?. exists x. eauto.
+Qed.
+
+Lemma SIMP_call_up_to_eq `{Encode X} (φ : X → Prop) v1 v2 v'2 :
+  SIMP (call v1 v2) φ →
+  v2 = v'2 →
+  SIMP (call v1 v'2) φ.
+Proof.
+  intros. subst. eauto.
+Qed.
+
+Lemma SIMP_call `{Encode X} `{Encode Y}
+  (φ : Y → Prop) v1 v'2 (x : X) :
+  v'2 = encode x →
+  SIMP (call v1 (encode x)) φ →
+  SIMP (call v1 v'2) φ.
+Proof.
+  intros. subst. eauto.
+Qed.
+
+Arguments String.eqb !s1 !s2 : simpl nomatch. (* TODO *)
+
+Notation "'<closure>'" := (VCloRec _ _ _) (only printing).
+Notation "'<closure>'" := (VClo _ _) (only printing).
+Notation "'Environment'  'composed'  'of'  [ x ; .. ; z ]" :=
+  (EnvCons x _ (.. (EnvCons z _ EnvNil) ..))
+ (only printing).
+
+(* WIP *)
+
+Create HintDb SIMP_specs.
+
+Ltac SIMP_call :=
+  eapply SIMP_covariant; [
+    notypeclasses refine (@SIMP_call _ _ _ _ _ _ _ _ _ _);
+      [ encode | eauto with SIMP_specs ]
+  | cbn
+  ].
 
 (* -------------------------------------------------------------------------- *)
 
@@ -32,6 +103,15 @@ Fixpoint encode_tree `{Encode A} (t : tree A) : val :=
 Local Instance Encode_tree `{Encode A} : Encode (tree A) :=
   { encode := encode_tree }.
 
+Lemma encode_tree_is_encode `{Encode A} :
+  ∀ (t : tree A),
+  encode_tree t = encode t.
+Proof.
+  eauto.
+Qed.
+
+Local Hint Resolve encode_tree_is_encode : encode.
+
 Lemma solve_encode_Leaf `{Encode A} t :
   Leaf = t →
   VConstant "Leaf" = encode t.
@@ -55,16 +135,6 @@ Proof.
 Qed.
 
 Local Hint Resolve solve_encode_Leaf solve_encode_Node : encode.
-
-Lemma encode_tree_is_encode `{Encode A} :
-  ∀ (xs : tree A),
-  encode_tree xs = encode xs.
-Proof.
-  reflexivity.
-Qed.
-
-Local Hint Extern 1 (_ = _) =>
-  repeat rewrite encode_tree_is_encode : encode.
 
 (* -------------------------------------------------------------------------- *)
 
@@ -104,6 +174,38 @@ Fixpoint encode_zipper `{Encode A} (z : zipper A) : val :=
 Local Instance Encode_zipper `{Encode A} : Encode (zipper A) :=
   { encode := encode_zipper }.
 
+Lemma encode_zipper_is_encode `{Encode A} :
+  ∀ (z : zipper A),
+  encode_zipper z = encode z.
+Proof.
+  eauto.
+Qed.
+
+Local Hint Resolve encode_zipper_is_encode : encode.
+
+(* The depth of a zipper. *)
+
+Fixpoint depth {A} (z : zipper A) : nat :=
+  match z with
+  | Root =>
+      0
+  | NodeL z1 x t2 =>
+      1 + depth z1
+  | NodeR t1 x z2 =>
+      1 + depth z2
+  end.
+
+Definition zlt {A} (z1 z2 : zipper A) :=
+  depth z1 < depth z2.
+
+Lemma zlt_wf {A} :
+  well_founded (@zlt A).
+Proof.
+  unfold zlt. eapply wf_inverse_image. eapply lt_wf.
+Qed.
+
+Local Hint Extern 1 (depth _ < depth _) => (simpl; lia) : SIMP_specs.
+
 (* -------------------------------------------------------------------------- *)
 
 (* WIP *)
@@ -126,41 +228,52 @@ Instance Encode_tuple4
       )
   }.
 
+Lemma solve_encode_tuple4
+  `{Encode A}
+  `{Encode B}
+  `{Encode C}
+  `{Encode D}
+  (a : A) (b : B) (c : C) (d : D)
+  ea eb ec ed
+  t :
+  (a, b, c, d) = t →
+  ea = encode a →
+  eb = encode b →
+  ec = encode c →
+  ed = encode d →
+  VTuple (
+    VCons ea $
+    VCons eb $
+    VCons ec $
+    VCons ed $
+    VNil
+  ) = encode t.
+Proof.
+  intros. subst. eauto.
+Qed.
+
+(* The lemma [solve_encode_tuple4] has 22 arguments. *)
+
+(* We cannot let [eapply] apply this lemma, as Coq would again make
+   incorrect choices of the types A, B, C, D. *)
+
+Hint Extern 1 (_ = _) =>
+  notypeclasses refine (@solve_encode_tuple4
+    _ _ _ _ _ _ _ _
+    _ _ _ _ _ _ _ _
+    _ _ _ _ _ _
+  )
+  : encode.
+
 (* -------------------------------------------------------------------------- *)
 
 (* Specification of [splay]. *)
 
 Definition splay_spec (splay : val) : Prop :=
-  ∀ `{Encode A} (l : tree A) (x : A) (r : tree A) (ctx : zipper A),
+  ∀ `{Encode A} (ctx : zipper A) (l : tree A) (x : A) (r : tree A),
   SIMP
     (call splay (encode (l, x, r, ctx)))
     (λ (t' : tree A), True).
-
-(* -------------------------------------------------------------------------- *)
-
-(* WIP *)
-
-Ltac SIMP_specify x φ :=
-  lazymatch goal with
-  | |- SIMP (bind (dconcatenating ?δ _) _) _ =>
-      let o := eval cbn in (lookup_name δ x) in
-      lazymatch o with ret ?v =>
-        let h := fresh in
-        assert (φ v) as h; [| revert h; generalize v ]
-      end
-  end.
-
-Lemma SIMP_simp_bind X Y (_ : Encode Y)
-   m f (x : X) (ψ : Y → Prop) :
-  simp m (ret x) →
-  SIMP (f x) ψ →
-  SIMP (bind m f) ψ.
-  (* This is [@bind X val]. *)
-Proof.
-  intros Hm Hf.
-  destruct Hf as (y & ? & ?).
-  eexists; split; eauto using prove_simp_bind.
-Qed.
 
 Lemma Splay__spec:
   let η := EnvCons "Stdlib" Stdlib EnvNil in
@@ -168,30 +281,67 @@ Lemma Splay__spec:
 Proof.
   intros.
   SIMP.
+
   SIMP_specify "splay" splay_spec.
   (* Subgoal: prove that [splay] satisfies its specification. *)
-  { unfold splay_spec. intros.
+  { unfold splay_spec. intros ??.
+    (* Reason by well-founded induction on the depth of the zipper [ctx]. *)
+    induction ctx as [ctx IH] using (well_founded_induction zlt_wf).
+    unfold zlt in IH.
+    intros.
+    (* Enter the closure. *)
     SIMP_enter. SIMP_continue.
-    (* Perform case analysis on the zipper [ctx]. *)
+    (* Optional: abstract away the closure; make it an abstract value [c]. *)
+    match type of IH with ∀ _ _ _ _ _, SIMP (call ?closure _) _ =>
+      revert IH; generalize closure; intros c IH
+    end.
+    (* Perform case analysis over the zipper [ctx]. *)
     destruct ctx as [| ctx y ry | ly y ctx ]; SIMP.
     (* Case: [Root]. *)
     { SIMP_continue.
-      (* For now, the postcondition is True. *)
+      (* Establish the postcondition. *)
       tauto. }
     (* Case: [NodeL]. *)
     { (* Perform case analysis on the second level of the zipper. *)
-      destruct ctx as [| lz z up | up z rz ]; SIMP; SIMP_continue.
+      destruct ctx as [| up z rz | lz z up ]; SIMP.
       (* Subcase: [Root]. *)
-      { (* For now, the postcondition is True. *)
+      { SIMP_continue.
+        (* Establish the postcondition. *)
         tauto. }
       (* Subcase: [NodeL]. *)
-      { admit. }
+      { SIMP_continue.
+        (* Apply the induction hypothesis. *)
+        SIMP_call; intros t'.
+        (* Establish the postcondition. *)
+        tauto. }
       (* Subcase: [NodeR]. *)
-      { admit. }
+      { SIMP_continue.
+        (* Apply the induction hypothesis. *)
+        SIMP_call; intros t'.
+        (* Establish the postcondition. *)
+        tauto. }
     }
     (* Case: [NodeR]. *)
-    { destruct ctx; admit.
+    { (* Perform case analysis on the second level of the zipper. *)
+      destruct ctx as [| up z rz | lz z up ]; SIMP.
+      (* Subcase: [Root]. *)
+      { SIMP_continue.
+        (* Establish the postcondition. *)
+        tauto. }
+      (* Subcase: [NodeL]. *)
+      { SIMP_continue.
+        (* Apply the induction hypothesis. *)
+        SIMP_call; intros t'.
+        (* Establish the postcondition. *)
+        tauto. }
+      (* Subcase: [NodeR]. *)
+      { SIMP_continue.
+        (* Apply the induction hypothesis. *)
+        SIMP_call; intros t'.
+        (* Establish the postcondition. *)
+        tauto. }
     }
   }
-  intros splay Hsplay. (* SIMP_continue. *)
-Abort.
+  intros splay Hsplay. SIMP_continue.
+
+Abort. (* unfinished; TODO *)
